compiler/core/EJson/Operators/EJsonSortBy.v
@@ -1,0 +1,97 @@
+(*
+ * Licensed under the Apache License, Version 2.0 (the "License");
+ * you may not use this file except in compliance with the License.
+ * You may obtain a copy of the License at
+ *
+ * http://www.apache.org/licenses/LICENSE-2.0
+ *
+ * Unless required by applicable law or agreed to in writing, software
+ * distributed under the License is distributed on an "AS IS" BASIS,
+ * WITHOUT WARRANTIES OR CONDITIONS OF ANY KIND, either express or implied.
+ * See the License for the specific language governing permissions and
+ * limitations under the License.
+ *)
+
+Require Import Orders.
+Require Import Equivalence.
+Require Import EquivDec.
+Require Import Compare_dec.
+Require Import Omega.
+Require Import String.
+Require Import List.
+Require Import ZArith.
+Require Import Utils.
+Require Import ForeignEJson.
+Require Import EJson.
+
+Section EJsonSortBy.
+  Context {fejson:foreign_ejson}.
+
+  Definition ejson_get_criteria (j:ejson) (sc:ejson) : option sdata :=
+    match sc with
+    | ejobject (("asc"%string, ejstring att)::nil)
+    | ejobject (("desc"%string, ejstring att)::nil) => (* XXX IGNORES sort kind (asc|desc) XXX *)
+      match ejson_is_record j with
+      | Some r =>
+        match edot r att with
+        | Some (ejbigint n) => Some (sdnat n)
+        | Some (ejstring s) => Some (sdstring s)
+        | Some _ => None
+        | None => None
+        end
+      | None => None
+      end
+    | _ => None
+    end.
+
+  Definition ejson_get_criterias (j:ejson) (scl:list ejson) : option (list sdata) :=
+    lift_map (ejson_get_criteria j) scl.
+
+  Definition ejson_sortable_data_of_ejson (j:ejson) (scl:list ejson) : option sortable_data :=
+    lift (fun c => (c,j)) (ejson_get_criterias j scl).
+
+  Definition ejson_sortable_coll_of_coll (scl:list ejson) (coll:list ejson) :
+    option (list sortable_data)
+    := lift_map (fun j => ejson_sortable_data_of_ejson j scl) coll.
+  
+  Definition ejson_sort (scl:list ejson) (j:ejson) : option ejson :=
+    match j with
+    | ejarray coll =>
+      lift ejarray
+           (lift coll_of_sortable_coll
+                 (lift sort_sortable_coll
+                       (ejson_sortable_coll_of_coll scl coll)))
+    | _ => None
+    end.
+
+  (* Example *)
+  Definition mkperson (name:string) (age:Z) (zip:Z) (company:string) :=
+    ejobject (("name", ejstring name)
+                :: ("age", ejbigint age)
+                :: ("zip", ejbigint zip)
+                :: ("company", ejstring company)
+                :: nil)%string.
+  Definition mkpersons_aux l :=
+    map (fun x =>
+           match x with (name, age, zip, company) => mkperson name age zip company
+           end) l.
+  Definition mkpersons l :=
+    ejarray (mkpersons_aux l).
+
+  Open Scope Z_scope.
+  Definition persons :=
+    mkpersons
+      (("John",23,1008,"ACME")
+         :: ("Jane",24,1009,"AIGO")
+         :: ("Jill",25,1010,"ACME")
+         :: ("Jack",27,1010,"CMUD")
+         :: nil)%string.
+
+  (*
+  Eval vm_compute in persons.
+  Eval vm_compute in (ejson_sort ((ejobject (("asc"%string,ejstring "name"%string)::nil)::nil)) persons).
+  Eval vm_compute in (ejson_sort ((ejobject (("asc"%string,ejstring "zip"%string)::nil))::(ejobject (("asc"%string, ejstring "name"%string)::nil))::nil) persons).
+  *)
+
+End EJsonSortBy.
+
