compiler/core/TypeSystem/RSubtypeProp.v
@@ -23,227 +23,227 @@ Require Export RSubtype.
 
 Section RSubtypeProp.
 
-Context {ftype:foreign_type}.
-Context {m:brand_relation}.
+  Context {ftype:foreign_type}.
+  Context {m:brand_relation}.
 
-Lemma top_subtype z : ⊤ <: z -> z = ⊤.
-Proof.
-  inversion 1; subst; eauto.
-Qed.
+  Lemma top_subtype z : ⊤ <: z -> z = ⊤.
+  Proof.
+    inversion 1; subst; eauto.
+  Qed.
 
-Lemma subtype_bottom z : z <: ⊥ -> z = ⊥.
-Proof.
-  inversion 1; subst; eauto.
-Qed.
+  Lemma subtype_bottom z : z <: ⊥ -> z = ⊥.
+  Proof.
+    inversion 1; subst; eauto.
+  Qed.
 
-Ltac simpl_type :=
-  repeat match goal with
-      | [H: ?z <: ⊥ |- _] => apply subtype_bottom in H; subst
-      | [H: ⊤ <: ?z |- _] => apply top_subtype in H; subst
-  end.
+  Ltac simpl_type :=
+    repeat match goal with
+           | [H: ?z <: ⊥ |- _] => apply subtype_bottom in H; subst
+           | [H: ⊤ <: ?z |- _] => apply top_subtype in H; subst
+           end.
 
-Instance subtype_trans : Transitive subtype.
-Proof.
-  Hint Constructors subtype.
-  red.
-  intros x y.
-  revert x.
-  induction y using rtype_rect; intros x z sub1 sub2; inversion sub1; subst; simpl_type; eauto.
-  - inversion sub2; subst; eauto.
-    rtype_equalizer. subst; eauto.
-  - inversion sub2; subst; eauto.
-    rtype_equalizer. subst.
-    constructor.
-    + intros s' r' lsr'.
-       destruct (H5 _ _  lsr') as [?[look3 sub3]].
-       destruct (H3 _ _ look3) as [?[??]].
-       exists x0; intuition.
-       generalize (Forallt_In H (s',x)). 
-       simpl; intros P; eapply P; eauto.
-       apply (lookup_in string_dec); trivial.
-    + intuition.
-  - inversion sub2; subst; eauto.
-    rtype_equalizer. subst. eauto.
-  - rtype_equalizer. subst.
-    inversion sub2; subst; trivial.
-    rtype_equalizer. subst.
-    econstructor; eauto.
-  - inversion sub2; subst; trivial.
-    apply canon_equiv in H; apply canon_equiv in H0.
-    rewrite H in H1.
-    rewrite H0 in H2.
-    constructor; etransitivity; eassumption.
-  - invcs sub2; trivial.
-    econstructor.
-    transitivity ft; trivial.
-Qed.
+  Instance subtype_trans : Transitive subtype.
+  Proof.
+    Hint Constructors subtype.
+    red.
+    intros x y.
+    revert x.
+    induction y using rtype_rect; intros x z sub1 sub2; inversion sub1; subst; simpl_type; eauto.
+    - inversion sub2; subst; eauto.
+      rtype_equalizer. subst; eauto.
+    - inversion sub2; subst; eauto.
+      rtype_equalizer. subst.
+      constructor.
+      + intros s' r' lsr'.
+        destruct (H5 _ _  lsr') as [?[look3 sub3]].
+        destruct (H3 _ _ look3) as [?[??]].
+        exists x0; intuition.
+        generalize (Forallt_In H (s',x)). 
+        simpl; intros P; eapply P; eauto.
+        apply (lookup_in string_dec); trivial.
+      + intuition.
+    - inversion sub2; subst; eauto.
+      rtype_equalizer. subst. eauto.
+    - rtype_equalizer. subst.
+      inversion sub2; subst; trivial.
+      rtype_equalizer. subst.
+      econstructor; eauto.
+    - inversion sub2; subst; trivial.
+      apply canon_equiv in H; apply canon_equiv in H0.
+      rewrite H in H1.
+      rewrite H0 in H2.
+      constructor; etransitivity; eassumption.
+    - invcs sub2; trivial.
+      econstructor.
+      transitivity ft; trivial.
+  Qed.
 
-Global Instance subtype_pre : PreOrder subtype.
-Proof.
-  constructor; eauto.
-  apply subtype_trans.
-Qed.
+  Global Instance subtype_pre : PreOrder subtype.
+  Proof.
+    constructor; eauto.
+    apply subtype_trans.
+  Qed.
 
-Lemma Rec_subtype_cons_weaken k s r l₁ pf pf2: 
-  Rec k ((s, r) :: l₁) pf <: Rec Open l₁ pf2.
-Proof.
-  apply SRec_open; intros.
-  simpl.
-  case_eq (string_dec s0 s); [intros ? ?; subst | eauto].
-  assert False; [|intuition].
-  rewrite domain_cons in pf.
-  apply is_list_sorted_NoDup in pf; [|apply StringOrder.lt_strorder].
-  inversion pf; subst. elim H3. 
-  eapply in_dom; eapply lookup_in; eauto.
-Qed.
+  Lemma Rec_subtype_cons_weaken k s r l₁ pf pf2: 
+    Rec k ((s, r) :: l₁) pf <: Rec Open l₁ pf2.
+  Proof.
+    apply SRec_open; intros.
+    simpl.
+    case_eq (string_dec s0 s); [intros ? ?; subst | eauto].
+    assert False; [|intuition].
+    rewrite domain_cons in pf.
+    apply is_list_sorted_NoDup in pf; [|apply StringOrder.lt_strorder].
+    inversion pf; subst. elim H3. 
+    eapply in_dom; eapply lookup_in; eauto.
+  Qed.
 
-Lemma Rec_subtype_cons_inv2 {k1 k2 s r l₁ l₂ pf pf2}: 
-  Rec k1 l₁ pf <: Rec k2 ((s, r) :: l₂) pf2 ->
-       exists pf', 
-         Rec k1 l₁ pf <: Rec Open l₂ pf'.
-Proof.
-  intros sub.
-  generalize pf2.
-  rewrite domain_cons, is_list_sorted_cons.
-  intros [pf' _].
-  rewrite (Rec_subtype_cons_weaken k2 s r l₂ pf2 pf') in sub.
-  eauto.
-Qed.
-
-Lemma Rec_subtype_cons_inv1_open {k1 k2 s r l₁ l₂ pf pf2}: 
-  Rec k1 ((s, r) :: l₁) pf <: Rec k2 l₂ pf2 ->
-     lookup string_dec l₂ s = None ->
-     k2 = Open.
-Proof.
-  intro rt.
-  destruct k2; trivial.
-  intros lo.
-  apply lookup_none_nin in lo.
-  elim lo.
-  generalize (SRec_closed_equiv_domain rt); intros inns.
-  simpl in inns.
-  destruct (inns s).
-  apply H; intuition.
-Qed.
-
-Lemma Rec_subtype_cons_inv1 {k1 k2 s r l₁ l₂ pf pf2}: 
-  Rec k1 ((s, r) :: l₁) pf <: Rec k2 l₂ pf2 ->
-    lookup string_dec l₂ s = None ->
-       exists pf', 
-         Rec k1 l₁ pf' <: Rec Open l₂ pf2.
-Proof.
-  intros rt lo.
-  generalize (Rec_subtype_cons_inv1_open rt lo); intros; subst.
-  inversion rt; subst; rtype_equalizer.
-  - destruct l₂; simpl in H2; try discriminate.
-    inversion H2; subst. rtype_equalizer.
-    subst. destruct p; simpl in *.
-    destruct (string_dec s s); intuition congruence.
-  - subst. destruct rl1; simpl in H0; try discriminate.
-    inversion H0; rtype_equalizer. subst.
-    destruct p; simpl in lo |- *.
-    generalize pf.
-    rewrite domain_cons, is_list_sorted_cons; simpl.
+  Lemma Rec_subtype_cons_inv2 {k1 k2 s r l₁ l₂ pf pf2}: 
+    Rec k1 l₁ pf <: Rec k2 ((s, r) :: l₂) pf2 ->
+                    exists pf', 
+                      Rec k1 l₁ pf <: Rec Open l₂ pf'.
+  Proof.
+    intros sub.
+    generalize pf2.
+    rewrite domain_cons, is_list_sorted_cons.
     intros [pf' _].
-    exists pf'.
-    apply SRec_open; intros s0 r0 ls0.
-    specialize (H2 _ _ ls0); simpl in H2.
-    destruct (string_dec s0 s); eauto.
-    destruct H2 as [? [inv _]].
-    inversion inv; subst. congruence.
-Qed.
+    rewrite (Rec_subtype_cons_weaken k2 s r l₂ pf2 pf') in sub.
+    eauto.
+  Qed.
 
-(** Note that unlike the biased inverses, since we are removing 
+  Lemma Rec_subtype_cons_inv1_open {k1 k2 s r l₁ l₂ pf pf2}: 
+    Rec k1 ((s, r) :: l₁) pf <: Rec k2 l₂ pf2 ->
+                                lookup string_dec l₂ s = None ->
+                                k2 = Open.
+  Proof.
+    intro rt.
+    destruct k2; trivial.
+    intros lo.
+    apply lookup_none_nin in lo.
+    elim lo.
+    generalize (SRec_closed_equiv_domain rt); intros inns.
+    simpl in inns.
+    destruct (inns s).
+    apply H; intuition.
+  Qed.
+
+  Lemma Rec_subtype_cons_inv1 {k1 k2 s r l₁ l₂ pf pf2}: 
+    Rec k1 ((s, r) :: l₁) pf <: Rec k2 l₂ pf2 ->
+                                lookup string_dec l₂ s = None ->
+                                exists pf', 
+                                  Rec k1 l₁ pf' <: Rec Open l₂ pf2.
+  Proof.
+    intros rt lo.
+    generalize (Rec_subtype_cons_inv1_open rt lo); intros; subst.
+    inversion rt; subst; rtype_equalizer.
+    - destruct l₂; simpl in H2; try discriminate.
+      inversion H2; subst. rtype_equalizer.
+      subst. destruct p; simpl in *.
+      destruct (string_dec s s); intuition congruence.
+    - subst. destruct rl1; simpl in H0; try discriminate.
+      inversion H0; rtype_equalizer. subst.
+      destruct p; simpl in lo |- *.
+      generalize pf.
+      rewrite domain_cons, is_list_sorted_cons; simpl.
+      intros [pf' _].
+      exists pf'.
+      apply SRec_open; intros s0 r0 ls0.
+      specialize (H2 _ _ ls0); simpl in H2.
+      destruct (string_dec s0 s); eauto.
+      destruct H2 as [? [inv _]].
+      inversion inv; subst. congruence.
+  Qed.
+
+  (** Note that unlike the biased inverses, since we are removing 
      an element from both sides, it is possible for k2 to be Closed *)
-Lemma Rec_subtype_cons_inv {k1 k2 s r1 r2 l₁ l₂ pf pf2}: 
-  Rec k1 ((s, r1) :: l₁) pf <: Rec k2 ((s, r2) :: l₂) pf2 ->
-  exists pf' pf2', 
-    Rec k1 l₁ pf' <: Rec k2 l₂ pf2'.
-Proof.
-  intros rt.
-  inversion rt; subst; rtype_equalizer; subst.
-  - repeat (exists (is_list_sorted_cons_inv _ pf)). reflexivity.
-  - destruct rl1; simpl in H0; try discriminate.
-    destruct rl2; simpl in H3; try discriminate.
-    inversion H0; inversion H3; clear H0; clear H3.
-    rtype_equalizer. subst.
-    exists (is_list_sorted_cons_inv _ pf).
-    exists (is_list_sorted_cons_inv _ pf2).
-    generalize (is_list_sorted_NoDup ODT_lt_dec _ pf).
-    generalize (is_list_sorted_NoDup ODT_lt_dec _ pf2).
-    intros.
-    constructor.
-    + intros. 
-      specialize (H2 s r').
-      simpl in H2.
-      destruct p; destruct p0; simpl in *; subst.
-      destruct (string_dec s s0).
-      * inversion H; subst.
-        apply lookup_in in H1.
-        apply in_dom in H1.
+  Lemma Rec_subtype_cons_inv {k1 k2 s r1 r2 l₁ l₂ pf pf2}: 
+    Rec k1 ((s, r1) :: l₁) pf <: Rec k2 ((s, r2) :: l₂) pf2 ->
+                                 exists pf' pf2', 
+                                   Rec k1 l₁ pf' <: Rec k2 l₂ pf2'.
+  Proof.
+    intros rt.
+    inversion rt; subst; rtype_equalizer; subst.
+    - repeat (exists (is_list_sorted_cons_inv _ pf)). reflexivity.
+    - destruct rl1; simpl in H0; try discriminate.
+      destruct rl2; simpl in H3; try discriminate.
+      inversion H0; inversion H3; clear H0; clear H3.
+      rtype_equalizer. subst.
+      exists (is_list_sorted_cons_inv _ pf).
+      exists (is_list_sorted_cons_inv _ pf2).
+      generalize (is_list_sorted_NoDup ODT_lt_dec _ pf).
+      generalize (is_list_sorted_NoDup ODT_lt_dec _ pf2).
+      intros.
+      constructor.
+      + intros. 
+        specialize (H2 s r').
+        simpl in H2.
+        destruct p; destruct p0; simpl in *; subst.
+        destruct (string_dec s s0).
+        * inversion H; subst.
+          apply lookup_in in H1.
+          apply in_dom in H1.
+          intuition.
+        * auto.
+      + intuition; subst.
+        destruct p; destruct p0; simpl in *; subst.
+        specialize (H5 s). intuition.
+        inversion H0; subst.
         intuition.
-      * auto.
-    + intuition; subst.
-       destruct p; destruct p0; simpl in *; subst.
-       specialize (H5 s). intuition.
-       inversion H0; subst.
-       intuition.
-Qed.
+  Qed.
 
-Global Instance subtype_part : PartialOrder eq subtype.
-Proof.
-  unfold PartialOrder, relation_equivalence, predicate_equivalence,
+  Global Instance subtype_part : PartialOrder eq subtype.
+  Proof.
+    unfold PartialOrder, relation_equivalence, predicate_equivalence,
     relation_conjunction, predicate_intersection, Basics.flip; simpl.
-  split; intros; subst; intuition.
-  revert x0 H0 H1.
-  induction x using rtype_rect; intros y sub1 sub2;
-  simpl_type; trivial;
-  inversion sub1; subst; simpl_type; trivial.
-  - f_equal. inversion sub2; subst;
-      rtype_equalizer.
-    + subst; eauto.
-    + subst; eauto.
-  - rtype_equalizer; subst.
-    intros.
-    apply rtype_fequal; simpl.
-    inversion sub2; rtype_equalizer; subst; try apply Rec_pr_irrel; auto 1.
-    f_equal; [ destruct k; destruct k2; intuition | ].
-    f_equal.
-    apply Forall2_eq.
-    assert (deq:domain srl = domain rl2) by
-     (eapply (@Sorted_incl_both_eq _ StringOrder.lt);
-     [ apply string_eqdec
-     | apply StringOrder.lt_strorder
-     | eapply is_list_sorted_Sorted_iff; eauto
-     | eapply is_list_sorted_Sorted_iff; eauto
-     | apply (SRec_closed_in_domain sub2)
-     | apply (SRec_closed_in_domain sub1)]).
-    revert k k2 rl2 pf2 H sub1 sub2 H2 H4 H5 H7 deq.
-    induction srl; destruct rl2; trivial; intros.
-    + destruct p. 
-      generalize (H2 s r); simpl.
-      destruct (string_dec s s); intuition.
-      destruct H1; intuition; discriminate.
-    + destruct a. 
-      generalize (H5 s r); simpl.
-      destruct (string_dec s s); intuition.
-      destruct H1; intuition; discriminate.
-    + inversion H; subst. destruct a; destruct p.
-       simpl in deq. inversion deq; subst; clear deq.
-       simpl in H3.
-       specialize (H3 r0).
-       specialize (H5 s0 r); specialize (H2 s0 r0).
-       simpl in H2, H5.
-       destruct (string_dec s0 s0); intuition.
-       destruct H0 as [? [eq1 su1]].
-       destruct H1 as [? [eq2 su2]].
-       inversion eq1; inversion eq2; subst.
-       intuition; subst.
-       
-       constructor; trivial.
-       destruct (Rec_subtype_cons_inv sub1) as [pf'11 [pf'12 sub'1]].
-       destruct (Rec_subtype_cons_inv sub2) as [pf'21 [pf'22 sub'2]].
-       eapply (IHsrl (is_list_sorted_cons_inv _ pf) k k2); trivial.
+    split; intros; subst; intuition.
+    revert x0 H0 H1.
+    induction x using rtype_rect; intros y sub1 sub2;
+      simpl_type; trivial;
+        inversion sub1; subst; simpl_type; trivial.
+    - f_equal. inversion sub2; subst;
+                 rtype_equalizer.
+      + subst; eauto.
+      + subst; eauto.
+    - rtype_equalizer; subst.
+      intros.
+      apply rtype_fequal; simpl.
+      inversion sub2; rtype_equalizer; subst; try apply Rec_pr_irrel; auto 1.
+      f_equal; [ destruct k; destruct k2; intuition | ].
+      f_equal.
+      apply Forall2_eq.
+      assert (deq:domain srl = domain rl2) by
+          (eapply (@Sorted_incl_both_eq _ StringOrder.lt);
+           [ apply string_eqdec
+           | apply StringOrder.lt_strorder
+           | eapply is_list_sorted_Sorted_iff; eauto
+           | eapply is_list_sorted_Sorted_iff; eauto
+           | apply (SRec_closed_in_domain sub2)
+           | apply (SRec_closed_in_domain sub1)]).
+      revert k k2 rl2 pf2 H sub1 sub2 H2 H4 H5 H7 deq.
+      induction srl; destruct rl2; trivial; intros.
+      + destruct p. 
+        generalize (H2 s r); simpl.
+        destruct (string_dec s s); intuition.
+        destruct H1; intuition; discriminate.
+      + destruct a. 
+        generalize (H5 s r); simpl.
+        destruct (string_dec s s); intuition.
+        destruct H1; intuition; discriminate.
+      + inversion H; subst. destruct a; destruct p.
+        simpl in deq. inversion deq; subst; clear deq.
+        simpl in H3.
+        specialize (H3 r0).
+        specialize (H5 s0 r); specialize (H2 s0 r0).
+        simpl in H2, H5.
+        destruct (string_dec s0 s0); intuition.
+        destruct H0 as [? [eq1 su1]].
+        destruct H1 as [? [eq2 su2]].
+        inversion eq1; inversion eq2; subst.
+        intuition; subst.
+        
+        constructor; trivial.
+        destruct (Rec_subtype_cons_inv sub1) as [pf'11 [pf'12 sub'1]].
+        destruct (Rec_subtype_cons_inv sub2) as [pf'21 [pf'22 sub'2]].
+        eapply (IHsrl (is_list_sorted_cons_inv _ pf) k k2); trivial.
         * erewrite (Rec_pr_irrel); eauto.
         * erewrite (Rec_pr_irrel _ _ pf'12).
           erewrite (Rec_pr_irrel _ _ (is_list_sorted_cons_inv ODT_lt_dec pf)).
@@ -252,99 +252,99 @@ Proof.
         * inversion sub'1; rtype_equalizer; subst; eauto.
         * inversion sub'2; rtype_equalizer; subst; eauto.
         * inversion sub'2; rtype_equalizer; subst; eauto.
-  - inversion sub2; subst; trivial;
-    rtype_equalizer; subst; trivial.
-    subst. f_equal; eauto.
-  - inversion sub2; subst; trivial;
-    rtype_equalizer; subst; trivial.
-    subst. f_equal; eauto.
-  - apply canon_equiv in H. rewrite H in H0.
-    apply rtype_fequal; simpl.
-    f_equal. apply canon_equiv. split; trivial.
-    inversion sub2; subst; trivial.
-    + apply canon_equiv in H3. destruct H3; trivial.
-    + apply canon_equiv in H1. apply canon_equiv in H2.
-      rewrite <- H1, <- H2; trivial.
-  - invcs sub2; trivial.
-    f_equal.
-    apply foreign_type_sub_part; split; trivial.
-Qed.
+    - inversion sub2; subst; trivial;
+        rtype_equalizer; subst; trivial.
+      subst. f_equal; eauto.
+    - inversion sub2; subst; trivial;
+        rtype_equalizer; subst; trivial.
+      subst. f_equal; eauto.
+    - apply canon_equiv in H. rewrite H in H0.
+      apply rtype_fequal; simpl.
+      f_equal. apply canon_equiv. split; trivial.
+      inversion sub2; subst; trivial.
+      + apply canon_equiv in H3. destruct H3; trivial.
+      + apply canon_equiv in H1. apply canon_equiv in H2.
+        rewrite <- H1, <- H2; trivial.
+    - invcs sub2; trivial.
+      f_equal.
+      apply foreign_type_sub_part; split; trivial.
+  Qed.
 
-Lemma wf_rtype_subtype_refl τ pf1 pf2:
-  exist (fun τ₀ : rtype₀ => wf_rtype₀ τ₀ = true) τ pf1 <:
-  exist (fun τ₀ : rtype₀ => wf_rtype₀ τ₀ = true) τ pf2.
-Proof.
-  generalize (wf_rtype₀_ext pf1 pf2); intros s.
-  subst. reflexivity.
-Qed.
+  Lemma wf_rtype_subtype_refl τ pf1 pf2:
+    exist (fun τ₀ : rtype₀ => wf_rtype₀ τ₀ = true) τ pf1 <:
+    exist (fun τ₀ : rtype₀ => wf_rtype₀ τ₀ = true) τ pf2.
+  Proof.
+    generalize (wf_rtype₀_ext pf1 pf2); intros s.
+    subst. reflexivity.
+  Qed.
 
-Lemma Rec_subtype_cons_eq {k₁ k₂ s r₁ r₂ rl₁ rl₂ pf1 pf2}  :
-      Rec k₁ ((s, r₁) :: rl₁) pf1 <: Rec k₂ ((s, r₂) :: rl₂) pf2 ->
-                                  r₁ <: r₂.
-Proof.
-  inversion 1; subst; rtype_equalizer.
-  subst; intros. reflexivity.
-  destruct rl1; try discriminate.
-  destruct rl2; try discriminate.
-  destruct p; destruct p0.
-  simpl in H1, H4.
-  inversion H1; subst.
-  inversion H4; subst.
-  rtype_equalizer. subst.
-  specialize (H3 s r₂).
-  simpl in H3.
-  destruct (string_dec s s); intuition.
-  destruct H0 as [? [inv sub]].
-  inversion inv; subst.
-  auto.
-Qed.
+  Lemma Rec_subtype_cons_eq {k₁ k₂ s r₁ r₂ rl₁ rl₂ pf1 pf2}  :
+    Rec k₁ ((s, r₁) :: rl₁) pf1 <: Rec k₂ ((s, r₂) :: rl₂) pf2 ->
+                                   r₁ <: r₂.
+  Proof.
+    inversion 1; subst; rtype_equalizer.
+    subst; intros. reflexivity.
+    destruct rl1; try discriminate.
+    destruct rl2; try discriminate.
+    destruct p; destruct p0.
+    simpl in H1, H4.
+    inversion H1; subst.
+    inversion H4; subst.
+    rtype_equalizer. subst.
+    specialize (H3 s r₂).
+    simpl in H3.
+    destruct (string_dec s s); intuition.
+    destruct H0 as [? [inv sub]].
+    inversion inv; subst.
+    auto.
+  Qed.
 
-Lemma STop₀ pf τ : τ <: exist (fun τ₀ : rtype₀ => wf_rtype₀ τ₀ = true) ⊤₀ pf.
-Proof.
-  generalize (STop τ).
-  destruct τ; unfold Top; intros.
-  eapply subtype_ext; eauto.
-Qed.
+  Lemma STop₀ pf τ : τ <: exist (fun τ₀ : rtype₀ => wf_rtype₀ τ₀ = true) ⊤₀ pf.
+  Proof.
+    generalize (STop τ).
+    destruct τ; unfold Top; intros.
+    eapply subtype_ext; eauto.
+  Qed.
 
-Lemma SBottom₀ pf τ : exist (fun τ₀ : rtype₀ => wf_rtype₀ τ₀ = true) ⊥₀ pf <: τ.
-Proof.
-  generalize (SBottom τ).
-  destruct τ; unfold Top; intros.
-  eapply subtype_ext; eauto.
-Qed.
+  Lemma SBottom₀ pf τ : exist (fun τ₀ : rtype₀ => wf_rtype₀ τ₀ = true) ⊥₀ pf <: τ.
+  Proof.
+    generalize (SBottom τ).
+    destruct τ; unfold Top; intros.
+    eapply subtype_ext; eauto.
+  Qed.
 
-Lemma SRefl₀ τ₀ pf : exist (fun τ₀ : rtype₀ => wf_rtype₀ τ₀ = true) τ₀ pf <: exist (fun τ₀ : rtype₀ => wf_rtype₀ τ₀ = true) τ₀ pf.
-Proof.
-  apply SRefl.
-Qed.
+  Lemma SRefl₀ τ₀ pf : exist (fun τ₀ : rtype₀ => wf_rtype₀ τ₀ = true) τ₀ pf <: exist (fun τ₀ : rtype₀ => wf_rtype₀ τ₀ = true) τ₀ pf.
+  Proof.
+    apply SRefl.
+  Qed.
 
-Lemma SColl₀ τ₁ pf₁ τ₂ pf₂ : 
-   exist (fun τ₀ : rtype₀ => wf_rtype₀ τ₀ = true) τ₁ pf₁ <: exist (fun τ₀ : rtype₀ => wf_rtype₀ τ₀ = true) τ₂ pf₂ ->
-   exist (fun τ₀ : rtype₀ => wf_rtype₀ τ₀ = true) (Coll₀ τ₁) pf₁ <: exist (fun τ₀ : rtype₀ => wf_rtype₀ τ₀ = true) (Coll₀ τ₂) pf₂.
-Proof.
-  apply SColl.
-Qed.
+  Lemma SColl₀ τ₁ pf₁ τ₂ pf₂ : 
+    exist (fun τ₀ : rtype₀ => wf_rtype₀ τ₀ = true) τ₁ pf₁ <: exist (fun τ₀ : rtype₀ => wf_rtype₀ τ₀ = true) τ₂ pf₂ ->
+                                                             exist (fun τ₀ : rtype₀ => wf_rtype₀ τ₀ = true) (Coll₀ τ₁) pf₁ <: exist (fun τ₀ : rtype₀ => wf_rtype₀ τ₀ = true) (Coll₀ τ₂) pf₂.
+  Proof.
+    apply SColl.
+  Qed.
 
-Lemma SRec₀ k1 rl1 rl2 k2 pf1 pf2 : (forall s r' pf',
-                      lookup string_dec rl2 s = Some r' -> 
-                      exists r pf, lookup string_dec rl1 s = Some r /\
-                                   subtype (exist _ r pf) (exist _ r' pf')) ->
-                                    (k2 = Closed -> k1 = Closed /\ 
-                                 (forall s, In s (domain rl1) -> In s (domain rl2))) ->
-exist (fun τ₀ : rtype₀ => wf_rtype₀ τ₀ = true) (Rec₀ k1 rl1) pf1 <:
-exist (fun τ₀ : rtype₀ => wf_rtype₀ τ₀ = true) (Rec₀ k2 rl2) pf2.
-Proof.
-  intros.
-  destruct (from_Rec₀ rl1 pf1) as [l1' [pf1' [eq11 eq12]]].
-  destruct (from_Rec₀ rl2 pf2) as [l2' [pf2' [eq21 eq22]]].
-  subst.
-  rewrite <- eq12, <- eq22.
-  apply SRec.
-  intros.
-  apply lookup_map_some in H1.
-  destruct (H s _ (proj2_sig r') H1) as [r [rpf [l1 s1]]].
-  exists (exist _ r rpf).
-  split.
+  Lemma SRec₀ k1 rl1 rl2 k2 pf1 pf2 : (forall s r' pf',
+                                          lookup string_dec rl2 s = Some r' -> 
+                                          exists r pf, lookup string_dec rl1 s = Some r /\
+                                                       subtype (exist _ r pf) (exist _ r' pf')) ->
+                                      (k2 = Closed -> k1 = Closed /\ 
+                                                      (forall s, In s (domain rl1) -> In s (domain rl2))) ->
+                                      exist (fun τ₀ : rtype₀ => wf_rtype₀ τ₀ = true) (Rec₀ k1 rl1) pf1 <:
+    exist (fun τ₀ : rtype₀ => wf_rtype₀ τ₀ = true) (Rec₀ k2 rl2) pf2.
+  Proof.
+    intros.
+    destruct (from_Rec₀ rl1 pf1) as [l1' [pf1' [eq11 eq12]]].
+    destruct (from_Rec₀ rl2 pf2) as [l2' [pf2' [eq21 eq22]]].
+    subst.
+    rewrite <- eq12, <- eq22.
+    apply SRec.
+    intros.
+    apply lookup_map_some in H1.
+    destruct (H s _ (proj2_sig r') H1) as [r [rpf [l1 s1]]].
+    exists (exist _ r rpf).
+    split.
     apply lookup_map_some; simpl. auto.
     destruct r'; simpl in *; auto.
 
@@ -353,39 +353,39 @@ Proof.
     unfold domain in H3; repeat rewrite map_map in H3.
     simpl in H3.
     auto.
-Qed.
+  Qed.
 
-Lemma subtype_Rec_sublist {k₁ l₁ pf₁ k₂ l₂ pf₂} :
-  Rec k₁ l₁ pf₁ <: Rec k₂ l₂ pf₂ -> sublist (domain l₂) (domain l₁).
-Proof.
-  inversion 1; subst; rtype_equalizer; subst; try reflexivity.
-  generalize pf₁ pf₂.
-  repeat rewrite sorted_StronglySorted by eapply StrictOrder_Transitive.
-  intros.
-  eapply StronglySorted_incl_sublist; eauto.
-  eapply SRec_closed_in_domain; eauto.
-Qed.
+  Lemma subtype_Rec_sublist {k₁ l₁ pf₁ k₂ l₂ pf₂} :
+    Rec k₁ l₁ pf₁ <: Rec k₂ l₂ pf₂ -> sublist (domain l₂) (domain l₁).
+  Proof.
+    inversion 1; subst; rtype_equalizer; subst; try reflexivity.
+    generalize pf₁ pf₂.
+    repeat rewrite sorted_StronglySorted by eapply StrictOrder_Transitive.
+    intros.
+    eapply StronglySorted_incl_sublist; eauto.
+    eapply SRec_closed_in_domain; eauto.
+  Qed.
 
 
-Lemma subtype_Rec_closed_domain {k₁ l₁ pf₁ l₂ pf₂} :
-  Rec k₁ l₁ pf₁ <: Rec Closed l₂ pf₂ -> (domain l₂) = (domain l₁).
-Proof.
-  intros sub.
-  apply Sorted_incl_both_eq; try eapply is_list_sorted_Sorted_iff; eauto
-  ;  intros; eapply (SRec_closed_equiv_domain sub); trivial.
-Qed.
+  Lemma subtype_Rec_closed_domain {k₁ l₁ pf₁ l₂ pf₂} :
+    Rec k₁ l₁ pf₁ <: Rec Closed l₂ pf₂ -> (domain l₂) = (domain l₁).
+  Proof.
+    intros sub.
+    apply Sorted_incl_both_eq; try eapply is_list_sorted_Sorted_iff; eauto
+    ;  intros; eapply (SRec_closed_equiv_domain sub); trivial.
+  Qed.
 
-Lemma subtype_Rec_closed2_closed1 {k1 l1 pf1 l2 pf2}:
-  Rec k1 l1 pf1 <: Rec Closed l2 pf2 ->
-                   k1 = Closed.
-Proof.
-  inversion 1; subst; intuition.
-Qed.
+  Lemma subtype_Rec_closed2_closed1 {k1 l1 pf1 l2 pf2}:
+    Rec k1 l1 pf1 <: Rec Closed l2 pf2 ->
+                     k1 = Closed.
+  Proof.
+    inversion 1; subst; intuition.
+  Qed.
 
   Lemma is_list_sorted_in_cons_lookup_none {B} {b τ₃ s} (τ₁:B) {rl0 rl1 τ₀} (τ₂:B) 
-   (pf1 : is_list_sorted ODT_lt_dec (domain ((b, τ₃) :: rl1)) = true)
-   (x : is_list_sorted ODT_lt_dec (domain ((s, τ₁) :: rl0)) = true)
-   (inn:In (b, τ₀) rl0) :
+        (pf1 : @is_list_sorted string _ ODT_lt_dec (domain ((b, τ₃) :: rl1)) = true)
+        (x : @is_list_sorted string _ ODT_lt_dec (domain ((s, τ₁) :: rl0)) = true)
+        (inn:In (b, τ₀) rl0) :
     lookup string_dec ((b, τ₂) :: rl1) s = None.
   Proof.
     apply (sorted_cons_in _ _ _ x) in inn.
@@ -395,12 +395,12 @@ Qed.
     inversion isl; subst.
     apply lookup_nin_none.
     rewrite domain_cons; trivial.
- Qed.
-    
+  Qed.
+  
   Lemma Rec_subtype_In  {rl0 pf0 rl1 pf1 b τ₁ τ₂} :
-   Rec Open rl0 pf0 <:
-   Rec Open rl1 pf1 ->
-   In (b, τ₁) rl0 -> In (b, τ₂) rl1 -> τ₁ <: τ₂.
+    Rec Open rl0 pf0 <:
+    Rec Open rl1 pf1 ->
+    In (b, τ₁) rl0 -> In (b, τ₂) rl1 -> τ₁ <: τ₂.
   Proof.
     revert rl0 pf0 pf1 b τ₁ τ₂. induction rl1; [simpl; intuition| ].
     intros.
@@ -411,9 +411,9 @@ Qed.
     - inversion H0; subst; clear H0.
       destruct H1.
       + inversion H0; subst; clear H0.
-         eapply Rec_subtype_cons_eq; eauto.
+        eapply Rec_subtype_cons_eq; eauto.
       + apply Rec_subtype_cons_inv2 in H.
-         destruct H. eapply (IHrl1 _ _ _ _ _ _ H); simpl; eauto.
+        destruct H. eapply (IHrl1 _ _ _ _ _ _ H); simpl; eauto.
     - destruct H1.
       + inversion H1; subst; clear H1.
         apply Rec_subtype_cons_inv1 in H.
@@ -421,15 +421,15 @@ Qed.
           revert H0 H. clear.
           revert rl1 b τ₁ τ₂  pf1 x. induction rl0; [simpl; intuition | ].
           intros.  simpl in H0. destruct H0; subst.
-            apply Rec_subtype_cons_eq in H; trivial.
-            destruct a.
-            apply Rec_subtype_cons_inv1 in H.
-            destruct H as [??].
-            eauto.
-            eapply is_list_sorted_in_cons_lookup_none; eauto.
+          apply Rec_subtype_cons_eq in H; trivial.
+          destruct a.
+          apply Rec_subtype_cons_inv1 in H.
+          destruct H as [??].
+          eauto.
+          eapply is_list_sorted_in_cons_lookup_none; eauto.
         * eapply is_list_sorted_in_cons_lookup_none; eauto.
       + rewrite  (Rec_subtype_cons_weaken Open s r rl1
-                                        pf1 (is_list_sorted_cons_inv _ pf1)) in H.
+                                          pf1 (is_list_sorted_cons_inv _ pf1)) in H.
         apply (IHrl1 _ _ _ b τ₁ τ₂ H); simpl; auto.
   Qed.
   
